FiatFormal/Language/Refinement.v
@@ -1,30 +1,134 @@
 
-(* Require Import FiatFormal.Language.Step. *)
+Require Import FiatFormal.Language.Step.
 
-(* (* need to access all operations of these adts. *) *)
-(* (* may need make use of wfP and wfADT to enforce n-ary. *) *)
-(* (* functions.  *) *)
 
-(* (* need way to specify method arity  *) *)
+Definition refines (x1 x2 : exp) :=
+  forall pb ds pbOK v,
+    STEPS pb ds pbOK x2 v
+    -> STEPS pb ds pbOK x1 v.
+Definition refinesP (p1 p2 : prog) :=
+  forall pb ds pbOK v,
+    STEPSP pb ds pbOK p2 v
+    -> STEPSP pb ds pbOK p1 v.
 
-(* Definition getRep (a : adt) := *)
+(* need to access all operations of these adts. *)
+(* may need make use of wfP and wfADT to enforce n-ary. *)
+(* functions.  *)
+
+(* need way to specify method arity  *)
+
+Definition getRep (a : adt) :=
+  match a with
+  | IADT r x s => r
+  end.
+Definition getBody (a : adt) :=
+  match a with
+  | IADT r x s => x
+  end.
+Definition getSig (a : adt) :=
+  match a with
+  | IADT r x s => s
+  end.
+
+(* Definition getArity (ts : list ty) (x : exp) (m : (XNFun ts x)) := *)
+(*   length ts. *)
+
+(* Definition getFuns := term. *)
+
+(* Definition getOps (a : adt) : list (option exp) := *)
 (*   match a with *)
-(*   | IADT r x s => r *)
-(*   end. *)
+(*   | IADT r x s => match x with *)
+(*                  | XTup xs => match xs with *)
+(*                                | ((XNFun ts x) as f) :: xs' => Some f :: (getOps a *)
+(*                                | _ :: xs' => *)
+(*                                | nil => nil *)
+(*                                end *)
+(*                  | _ => nil *)
+(*                                                                          end. *)
 
-(* (* Definition getOps (a : adt) := *) *)
-(* (*   match a with *) *)
-(* (*   | IADT r x s => match x with *) *)
-(* (*                  | TNProd xs => match xs with *) *)
-(* (*                                | TNFun ts tRes x :: xs' =>  *) *)
+(* Definition getMethods (a : adt) : list method := *)
+(* match a with *)
+(* | IADT r ms ts => ms *)
+(* end. *)
+
+(* Definition getArity (m : method) := *)
+(* match m with. *)
+
+(* Definition refinesADT (aOld aNew : adt) := *)
+(*   getBody aOld = (XTup ms) *)
+(*   -> Forall2 (fun m => exists ts x, m = (XNFun ts x)) ms *)
+(*   exists (absRel : getRep aOld -> getRep aNew -> Prop), *)
+(*     -> length ms = n *)
+(*     -> *)
+
+(*   forall methodsOld methodsNew methodOld methodNew i numMethods, *)
+(*     getMethods aOld = methodsOld *)
+(*     -> getMethods aNew = methodsNew *)
+(*     -> length methodsOld = length methodsNew *)
+(*     -> get i methodsNew = methodNew *)
+(*     -> get i methodsOld = methodOld *)
+(*     -> forall (reps_o : list (getRep aOld)) (reps_n : list (getRep aNew)) *)
+(*         (arity : nat) (domSize : nat) xs vPairNew vRes vPairOld rep_n', *)
+(*         arity = getArity methodNew *)
+(*         -> length reps_o = arity *)
+(*         -> length reps_n = arity *)
+(*         -> length xs = domSize *)
+(*         -> Forall2 (absRel) reps_o reps_n *)
+(*         -> STEPS (XNApp opNew (reps_n >< xs)) vPairNew *)
+(*         -> XProj 0 vPairNew = rep_n' *)
+(*         -> XProj 1 vPairNew = vRes *)
+(*         -> exists rep_o', *)
+(*             (STEPS (XNApp opOld (reps_o >< xs)) vPairOld *)
+(*             /\ XProj 0 vPairOld = rep_o' *)
+(*             /\ XProj 1 vPairOld = vRes) *)
+(*             /\ absRel rep_o' rep_n'. *)
 
 (* Definition ADTrefines (aOld aNew : adt) := *)
+(*   wfADT aOld -> wfADT aNew -> *)
 (*   exists (absRel : getRep aOld -> getRep aNew -> Prop), *)
-(*   forall op, *)
-(*     In op (getOps aOld) *)
-(*        forall (reps_o : getRep aOld) (reps_n : getRep aNew) len, *)
-(*          len = getArity op *)
-(*          -> length reps_o = len *)
-(*          -> length reps_n = len *)
-(*          -> Forall2 (absRel) reps_o reps_n *)
-(*          -> . *)
+(*   forall methodsOld methodsNew methodOld methodNew i numMethods, *)
+(*     getMethods aOld = methodsOld *)
+(*     -> getMethods aNew = methodsNew *)
+(*     -> length methodsOld = length methodsNew *)
+(*     -> get i methodsNew = methodNew *)
+(*     -> get i methodsOld = methodOld *)
+(*     -> forall (reps_o : list (getRep aOld)) (reps_n : list (getRep aNew)) *)
+(*         (arity : nat) (domSize : nat) xs vPairNew vRes vPairOld rep_n', *)
+(*         arity = getArity methodNew *)
+(*         -> length reps_o = arity *)
+(*         -> length reps_n = arity *)
+(*         -> length xs = domSize *)
+(*         -> Forall2 (absRel) reps_o reps_n *)
+(*         -> STEPS (XNApp opNew (reps_n >< xs)) vPairNew *)
+(*         -> XProj 0 vPairNew = rep_n' *)
+(*         -> XProj 1 vPairNew = vRes *)
+(*         -> exists rep_o', *)
+(*             (STEPS (XNApp opOld (reps_o >< xs)) vPairOld *)
+(*             /\ XProj 0 vPairOld = rep_o' *)
+(*             /\ XProj 1 vPairOld = vRes) *)
+(*             /\ absRel rep_o' rep_n'. *)
+
+
+(* Definition ADTrefines' (aOld aNew : adt) := *)
+(*   exists (absRel : getRep aOld -> getRep aNew -> Prop), *)
+(*   forall opsOld opsNew opOld opNew i numMethods, *)
+(*     getOps aOld = opsOld *)
+(*     -> getOps aNew = opsNew *)
+(*     -> length opsOld = length opsNew *)
+(*     -> get i opsNew = opNew *)
+(*     -> get i opsOld = opOld *)
+(*     -> forall (reps_o : list (getRep aOld)) (reps_n : list (getRep aNew)) *)
+(*         (arity : nat) (domSize : nat) xs vPairNew vRes vPairOld rep_n', *)
+(*         arity = getArity opNew *)
+(*         -> length reps_o = arity *)
+(*         -> length reps_n = arity *)
+(*         -> length xs = domSize *)
+(*         -> Forall2 (absRel) reps_o reps_n *)
+(*         -> STEPS (XNApp opNew (reps_n >< xs)) vPairNew *)
+(*         -> XProj 0 vPairNew = rep_n' *)
+(*         -> XProj 1 vPairNew = vRes *)
+(*         -> exists rep_o', *)
+(*             (STEPS (XNApp opOld (reps_o >< xs)) vPairOld *)
+(*             /\ XProj 0 vPairOld = rep_o' *)
+(*             /\ XProj 1 vPairOld = vRes) *)
+(*             /\ absRel rep_o' rep_n'. *)
