FiatFormal/Language/StepContext.v
@@ -1,0 +1,63 @@
+
+Require Import FiatFormal.Language.SubstTypeExp.
+Require Import FiatFormal.Language.SubstExpExp.
+Require Import FiatFormal.Language.Exp.
+
+Require Export FiatFormal.Data.Context.
+Require Export FiatFormal.Data.Chain.
+
+(* TODO: consider implications of below definition...
+         esp. that nary function application requires
+         value of function but only wnfX of args *)
+
+(*  Evaluation contexts for expressions.
+    This describes a place in the exp AST where the sub-expression
+    there is able to take an evaluation step *)
+Inductive exp_ctx : (exp -> exp) -> Prop :=
+
+ (* Left of an application *)
+ | XcApp1
+   : forall x2,
+     exp_ctx (fun xx => XApp xx x2)
+
+ (* The right of an application can step only when the left is
+    already a value. *)
+ | XcApp2
+   : forall v1,
+     value v1
+     -> exp_ctx (fun xx => XApp v1 xx)
+
+ | XcCon
+   : forall dc C,
+     exps_ctx wnfX C
+     -> exp_ctx (fun xx => XCon dc (C xx))
+
+ (* We need to reduce the discriminant of a match to a value. *)
+ | XcMatch
+   : forall alts,
+     exp_ctx (fun xx => XMatch xx alts)
+
+ | XcChoice
+   : forall t pc C,
+     exps_ctx wnfX C
+     -> exp_ctx (fun xx => XChoice t pc (C xx))
+
+ | XcTup
+   : forall C,
+     exps_ctx wnfX C
+     -> exp_ctx (fun xx => XTup (C xx))
+
+ | XcProj
+   : forall n,
+     exp_ctx (fun xx => XProj n xx)
+
+ | XcNApp1
+   : forall xs,
+     exp_ctx (fun xx => XNApp xx xs)
+
+ | XcNApp2
+   : forall v1 C,
+     value v1
+     -> exps_ctx wnfX C
+     -> exp_ctx (fun xx => XNApp v1 (C xx)).
+Hint Constructors exp_ctx.
